@prefix owl: <http://www.w3.org/2002/07/owl#> .
@prefix prov: <http://www.w3.org/ns/prov#> .
@prefix provs: <http://www.bosch.com/semantics/prov-star#> .
@prefix rdfs: <http://www.w3.org/2000/01/rdf-schema#> .
@prefix xsd: <http://www.w3.org/2001/XMLSchema#> .

<http://www.bosch.com/semantics/prov-star>
  a owl:Ontology ;
  owl:imports <http://www.w3.org/ns/prov-o#> ;
  owl:versionInfo "Version 1.0. Created by Henrik Dibowski" ;
.
provs:Query
  a owl:Class ;
  rdfs:label "Query" ;
  rdfs:subClassOf prov:Entity ;
.
provs:TripleChangeSet
  a owl:Class ;
  rdfs:comment "The set of triples changed during some graph update operation will be captured by the two subclasses of TripleChangeSet" ;
  rdfs:label "Triple Change Set" ;
  rdfs:subClassOf prov:Entity ;
.
provs:TripleGenerationSet
  a owl:Class ;
  rdfs:comment "Represents a set of triples created during some graph update operation. They will refer to the same TripleGenerationSet via statement-level annotations (RDF*)." ;
  rdfs:label "Triple Generation Set" ;
  rdfs:subClassOf provs:TripleChangeSet ;
.
provs:TripleInvalidationSet
  a owl:Class ;
  rdfs:comment "Represents a set of triples deleted during some graph update operation. They will refer to the same TripleInvalidationSet via statement-level annotations (RDF*)." ;
  rdfs:label "Triple Invalidation Set" ;
  rdfs:subClassOf provs:TripleChangeSet ;
.
provs:belongsTo
  a owl:AnnotationProperty ;
  rdfs:comment "for relating triples as quoted triples to TripleGenerationSet and TripleInvalidationSet instances (statement-level annotation using RDF*)" ;
  rdfs:label "belongs to" ;
  rdfs:range provs:TripleChangeSet ;
.
provs:queryString
  a owl:DatatypeProperty ;
  rdfs:domain provs:Query ;
  rdfs:label "query string" ;
  rdfs:range xsd:string ;
.
